more

thys/Substitution/Expression_Like.thy
@@ -1,204 +1,9 @@
 theory Expression_Like
-  imports "Binders.MRBNF_Recursor"
+  imports Underlying_MN_Monad
 begin
 
 (**************************)
-(* 1. Preliminaries *)
-
-declare supp_id_bound[simp] supp_inv_bound[simp] infinite_UNIV[simp]
-
-definition "IImsupp' Inj Vr \<rho> = SSupp Inj \<rho> \<union> IImsupp Inj Vr \<rho>"
-
-term curry
-definition "uncurry f \<equiv> \<lambda>(a,b). f a b" 
-lemma uncorry_apply[simp]: "uncurry f (a,b) = f a b"
-  unfolding uncurry_def by auto
-
-lemma fst_comp_id[simp]: "fst \<circ> (\<lambda>e. (e, p)) = id" by auto
-
-lemma tri_Un1: "A \<subseteq> B \<union> C \<Longrightarrow> A \<union> B \<subseteq> B \<union> C" by auto
-lemma tri_Un3: "A \<union> A' \<union> A'' \<subseteq> B \<union> C \<Longrightarrow> B \<union> A \<union> A' \<union> A'' \<subseteq> B \<union> C" by auto
-
-lemma A_Int_Un_emp: "A \<inter> (B \<union> C) = {} \<longleftrightarrow> A \<inter> B = {} \<and> A \<inter> C = {}" by auto
-
-lemma bij_inv_Un_triv: "bij \<sigma> \<Longrightarrow> \<sigma> ` A \<inter> B = {} \<longleftrightarrow> A \<inter> inv \<sigma> ` B = {}"
-  by (metis bij_def empty_is_image image_Int image_inv_f_f surj_imp_inj_inv)
-
-lemma bij_in_inv_Un_triv: "bij \<sigma> \<Longrightarrow> inv \<sigma> a \<in> B \<longleftrightarrow> a \<in> \<sigma> ` B"
-  by (metis bij_inv_eq_iff imageE image_eqI)
-
-lemma incl_Un_triv3: "A1 \<union> A2 \<union> A3 \<subseteq> A \<Longrightarrow> A1 \<subseteq> A \<and> A2 \<subseteq> A \<and> A3 \<subseteq> A" by auto
-
-lemma incl_Un3_triv3: "A1 \<subseteq> B1 \<Longrightarrow> A2 \<subseteq> B2 \<union> P \<Longrightarrow> A3 \<subseteq> B3 \<union> P \<Longrightarrow> A1 \<union> A2 \<union> A3 \<subseteq> B1 \<union> B2 \<union> B3 \<union> P" 
-by auto
-
-lemma triv_Un4_remove: "A1 \<union> A2 \<union> A3 \<subseteq> B1 \<union> B2 \<union> B3 \<union> P \<Longrightarrow> A1 \<union> A2 \<union> A3 \<union> P \<subseteq> B1 \<union> B2 \<union> B3 \<union> P"
-by auto
-
-definition small :: "('a::var \<Rightarrow> 'a) \<Rightarrow> bool" where 
-"small \<sigma> \<equiv> countable (supp \<sigma>)" 
-
-declare supp_id[simp,intro] (*: "supp id = {}" unfolding supp_def by auto *)
-lemma small_id[simp,intro]: "small id" unfolding small_def by auto
-lemma supp_id'[simp,intro]: "supp (\<lambda>a. a) = {}" unfolding supp_def by auto
-lemma small_id'[simp,intro]: "small (\<lambda>a. a)" unfolding small_def by auto
-
-thm supp_o
-(* lemma supp_o: "supp (\<sigma> o \<tau>) \<subseteq> supp \<sigma> \<union> supp \<tau>" unfolding supp_def by auto *)
-lemma small_o[simp]: "small \<sigma> \<Longrightarrow> small \<tau> \<Longrightarrow> small (\<sigma> o \<tau>)" 
-unfolding small_def using supp_o by (metis countable_Un_iff countable_subset)
-
-lemma supp_inv[simp]: "bij \<sigma> \<Longrightarrow> small \<sigma> \<Longrightarrow> supp (inv \<sigma>) = supp \<sigma>" 
-unfolding supp_def by (metis bij_inv_eq_iff)
-lemma small_inv[simp]: "bij \<sigma> \<Longrightarrow> small (inv \<sigma>) \<longleftrightarrow> small \<sigma>" 
-unfolding small_def by (metis bij_betw_inv_into inv_inv_eq small_def supp_inv)
-
-(* declare bij_id[intro] *)
-lemmas bij_id'[simp,intro]=bij_id[unfolded id_def]
-(* declare bij_comp[simp] *)
-(* declare bij_imp_bij_inv[simp] *)
-
-lemmas bij_inv_id1 = inv_o_simp2 (* [simp] *) (* : "bij f \<Longrightarrow> f o inv f = id" unfolding fun_eq_iff *)
- (*  by (simp add: bij_def surj_iff) *)
-lemmas bij_inv_id2 = inv_o_simp1 
-(*[simp]: "bij f \<Longrightarrow> inv f o f = id" unfolding fun_eq_iff 
-by (simp add: bij_def surj_iff) *)
-
-(**************************)
-(* 2. The starting MN-monad / pre-(co)datatype *)
-
-typedecl Gbd_type
-consts Gbd :: "Gbd_type rel"
-
-setup \<open>Sign.mandatory_path "G"\<close>
-axiomatization where
-  infinite_regular_card_order: "infinite_regular_card_order Gbd"
-setup \<open>Sign.parent_path\<close>
-
-class covar =
-  assumes large: "cardSuc Gbd \<le>o |UNIV::'a set|"
-    and regular: "regularCard |UNIV::'a set|"
-
-class var =
-  assumes large: "|Field Gbd| \<le>o |UNIV::'a set|"
-    and regular: "regularCard |UNIV::'a set|"
-
-instantiation Gbd_type :: var begin
-instance apply standard
-  apply simp
-  by (meson G.infinite_regular_card_order card_of_unique
-      card_order_on_Card_order infinite_regular_card_order_def
-      regularCard_ordIso)
-end
-
-subclass (in covar) var
-  apply standard
-  apply (meson cardSuc_ordLess_ordLeq card_of_Card_order
-      card_of_Field_ordIso G.infinite_regular_card_order
-      infinite_regular_card_order.Card_order local.large
-      ordIso_ordLeq_trans ordLeq_iff_ordLess_or_ordIso)
-  by (rule local.regular)
-
-subclass (in var) infinite
-  apply standard
-  using card_of_ordLeq_finite cinfinite_def
-    G.infinite_regular_card_order
-    infinite_regular_card_order.cinfinite local.large
-  by auto
-
-lemma large': "Gbd \<le>o |UNIV::'a::var set|"
-  using Card_order_iff_ordLeq_card_of var_class.large
-    G.infinite_regular_card_order infinite_regular_card_order.Card_order ordLeq_transitive
-  by blast
-
-lemma (in var) UN_bound: "|A| <o |UNIV::'a set| \<Longrightarrow> (\<And>x. x \<in> A \<Longrightarrow> |f x| <o |UNIV::'a set| )
-  \<Longrightarrow> |\<Union>(f ` A)| <o |UNIV::'a set|"
-  using card_of_Card_order card_of_UNION_ordLess_infinite_Field local.regular regularCard_stable
-  by (metis Field_card_of infinite_UNIV)
-
-lemma IImsupp_bound[simp]:
-  "|SSupp Inj (\<rho> :: 'a::var \<Rightarrow> _)| <o |UNIV :: 'a set| \<Longrightarrow> (\<And>x. |Vr (\<rho> x)| <o |UNIV :: 'a set| ) \<Longrightarrow>
-  |IImsupp' Inj (Vr :: _ \<Rightarrow> 'a set) \<rho>| <o |UNIV :: 'a set|"
-  unfolding IImsupp_def IImsupp'_def
-  by (auto simp: Un_bound UN_bound)
-
-typedecl ('a1, 'a2, 'c1, 'c2) G
-consts Gsub :: "('a1 :: var \<Rightarrow> 'a1) \<Rightarrow> ('a2 :: var \<Rightarrow> 'a2) \<Rightarrow> ('a1, 'a2, 'c1, 'c2) G \<Rightarrow> ('a1, 'a2, 'c1, 'c2) G"
-consts GVrs1 :: "('a1 :: var, 'a2 :: var, 'c1, 'c2) G \<Rightarrow> 'a1 set"
-consts GVrs2 :: "('a1 :: var, 'a2 :: var, 'c1, 'c2) G \<Rightarrow> 'a2 set"
-consts Gmap :: "('c1 \<Rightarrow> 'c1') \<Rightarrow> ('c2 \<Rightarrow> 'c2') \<Rightarrow> ('a1, 'a2, 'c1, 'c2) G \<Rightarrow> ('a1, 'a2, 'c1', 'c2') G"
-consts GSupp1 :: "('a1 :: var, 'a2 :: var, 'c1, 'c2) G \<Rightarrow> 'c1 set"
-consts GSupp2 :: "('a1 :: var, 'a2 :: var, 'c1, 'c2) G \<Rightarrow> 'c2 set"
-
-setup \<open>Sign.mandatory_path "G"\<close>
-
-axiomatization where
-  Sb_Inj: "Gsub id id = id" and
-  Sb_comp: "\<And>g1 g2 f1 f2.
-       |supp (f1 :: 'a1::var \<Rightarrow> 'a1)| <o |UNIV :: 'a1 set| \<Longrightarrow>
-       |supp (f2 :: 'a2::var \<Rightarrow> 'a2)| <o |UNIV :: 'a2 set| \<Longrightarrow>
-       |supp (g1 :: 'a1::var \<Rightarrow> 'a1)| <o |UNIV :: 'a1 set| \<Longrightarrow>
-       |supp (g2 :: 'a2::var \<Rightarrow> 'a2)| <o |UNIV :: 'a2 set| \<Longrightarrow>
-       Gsub g1 g2 \<circ> Gsub f1 f2 = Gsub (g1 \<circ> f1) (g2 \<circ> f2)" and
-  Vrs1_bd: "(\<And>x. |GVrs1 x| <o Gbd)" and
-  Vrs2_bd: "(\<And>x. |GVrs2 x| <o Gbd)" and
-  Vrs1_Sb: "(\<And>f1 f2 x.
-       |supp (f1 :: 'a1::var \<Rightarrow> 'a1)| <o |UNIV :: 'a1 set| \<Longrightarrow>
-       |supp (f2 :: 'a2::var \<Rightarrow> 'a2)| <o |UNIV :: 'a2 set| \<Longrightarrow> GVrs1 (Gsub f1 f2 x) = f1 ` GVrs1 x)" and
-  Vrs2_Sb: "(\<And>f1 f2 x.
-       |supp (f1 :: 'a1::var \<Rightarrow> 'a1)| <o |UNIV :: 'a1 set| \<Longrightarrow>
-       |supp (f2 :: 'a2::var \<Rightarrow> 'a2)| <o |UNIV :: 'a2 set| \<Longrightarrow> GVrs2 (Gsub f1 f2 x) = f2 ` GVrs2 x)" and
-  Sb_cong: "\<And>f1 f2 g1 g2 x.
-       |supp (f1 :: 'a1::var \<Rightarrow> 'a1)| <o |UNIV :: 'a1 set| \<Longrightarrow>
-       |supp (f2 :: 'a2::var \<Rightarrow> 'a2)| <o |UNIV :: 'a2 set| \<Longrightarrow>
-       |supp (g1 :: 'a1::var \<Rightarrow> 'a1)| <o |UNIV :: 'a1 set| \<Longrightarrow>
-       |supp (g2 :: 'a2::var \<Rightarrow> 'a2)| <o |UNIV :: 'a2 set| \<Longrightarrow>
-       (\<And>a1. a1 \<in> GVrs1 x \<Longrightarrow> f1 a1 = g1 a1) \<Longrightarrow>
-       (\<And>a2. a2 \<in> GVrs2 x \<Longrightarrow> f2 a2 = g2 a2) \<Longrightarrow>
-       Gsub f1 f2 x = Gsub g1 g2 x" and
-  Map_id: "Gmap id id = id" and
-  Map_comp: "\<And>f1 f2 g1 g2. Gmap g1 g2 \<circ> Gmap f1 f2 = Gmap (g1 \<circ> f1) (g2 \<circ> f2)" and
-  Supp1_Map: "(\<And>f1 f2 x. GSupp1 (Gmap f1 f2 x) = f1 ` GSupp1 x)" and
-  Supp2_Map: "(\<And>f1 f2 x. GSupp2 (Gmap f1 f2 x) = f2 ` GSupp2 x)" and
-  Supp1_bd: "(\<And>x. |GSupp1 x| <o Gbd)" and
-  Supp2_bd:  "(\<And>x. |GSupp2 x| <o Gbd)" and
-  Map_cong: "\<And>f1 f2 g1 g2 x.
-        (\<And>a. a \<in> GSupp1 x \<Longrightarrow> f1 a = g1 a) \<Longrightarrow>
-        (\<And>a. a \<in> GSupp2 x \<Longrightarrow> f2 a = g2 a) \<Longrightarrow>
-        Gmap f1 f2 x = Gmap g1 g2 x" and
-  Map_Sb: "\<And>f1 f2 g1 g2.
-        |supp (g1 :: 'a1::var \<Rightarrow> 'a1)| <o |UNIV :: 'a1 set| \<Longrightarrow>
-        |supp (g2 :: 'a2::var \<Rightarrow> 'a2)| <o |UNIV :: 'a2 set| \<Longrightarrow>
-        Gmap f1 f2 \<circ> Gsub g1 g2 = Gsub g1 g2 \<circ> Gmap f1 f2" and
-  Supp1_Sb: "(\<And>g1 g2 x.
-        |supp (g1 :: 'a1::var \<Rightarrow> 'a1)| <o |UNIV :: 'a1 set| \<Longrightarrow>
-        |supp (g2 :: 'a2::var \<Rightarrow> 'a2)| <o |UNIV :: 'a2 set| \<Longrightarrow> GSupp1 (Gsub g1 g2 x) = GSupp1 x)" and
-  Supp2_Sb:"(\<And>g1 g2 x.
-        |supp (g1 :: 'a1::var \<Rightarrow> 'a1)| <o |UNIV :: 'a1 set| \<Longrightarrow>
-        |supp (g2 :: 'a2::var \<Rightarrow> 'a2)| <o |UNIV :: 'a2 set| \<Longrightarrow> GSupp2 (Gsub g1 g2 x) = GSupp2 x)" and
-  Vrs_Map1: "(\<And>f1 f2 x. GVrs1 (Gmap f1 f2 x) = GVrs1 x)" and
-  Vrs_Map2: "(\<And>f1 f2 x. GVrs2 (Gmap f1 f2 x) = GVrs2 x)"
-
-lemmas Vrs_Sb = G.Vrs1_Sb G.Vrs2_Sb
-lemmas Vrs_bd = G.Vrs1_bd G.Vrs2_bd
-lemmas Supp_Map = G.Supp1_Map G.Supp2_Map
-lemmas Supp_bd = G.Supp1_bd G.Supp2_bd
-lemmas Supp_Sb = G.Supp1_Sb G.Supp2_Sb
-lemmas Vrs_Map = G.Vrs_Map1 G.Vrs_Map2
-
-setup \<open>Sign.parent_path\<close>
-
-(* In this case the flat version, Gren, happens to be the same as Gsub. *)
-definition Gren :: 
-  "('a1 :: var \<Rightarrow> 'a1) \<Rightarrow> ('a2 :: var \<Rightarrow> 'a2) \<Rightarrow> ('a1, 'a2, 'c1, 'c2) G \<Rightarrow> ('a1, 'a2, 'c1, 'c2) G" where 
-  "Gren \<rho>1 \<rho>2 u = Gsub \<rho>1 \<rho>2 u"
-
-lemma GVrs2_bound[simp]: "|GVrs2 (u::('a :: var, 'a, 'e, 'e) G)| <o |UNIV :: 'a set|"
-  by (rule ordLess_ordLeq_trans[OF G.Vrs_bd(2) large'])
-
-
-(**************************)
-(* 3. Generalized Nominal Assumptions *)
+(* 1. Generalized Nominal Assumptions *)
 
 locale Nominal = 
   fixes Eperm :: "('a :: var \<Rightarrow> 'a) \<Rightarrow> 'e \<Rightarrow> 'e"
@@ -229,7 +34,7 @@ lemma EVrs_bound[simp]: "|EVrs (x :: 'e)| <o |UNIV :: 'a set|"
 
 end
 
-(* relativized nominal :*)
+(* Relativized nominal :*)
 locale NominalRel = 
   fixes Pvalid :: "'e \<Rightarrow> bool"
   and Pperm :: "('a :: var \<Rightarrow> 'a) \<Rightarrow> 'e \<Rightarrow> 'e"
@@ -247,7 +52,28 @@ locale NominalRel =
 
 
 (**************************)
-(* 4. Expression-Like Entities *)
+(* 2. Expression-Like Entities *)
+
+(* In addition to the nominal structure, 
+expression also have a well-behaved 
+(in particular quasi-injective) 
+bindeing-aware constructor *)
+
+(* Recall that our G stands G0 in the 
+triple (I0,P0,G0), where  
+where I0 = {1,2} and P0 = {1,2}*)
+
+(* Below, the assumption is that, in  ('a,'a,'e,'e) G:
+-- the first-component-variables (GVrs1) are top-free 
+-- the second-conponent variables (GVrs2) are top-bound. 
+So in the binding-spec B = (J0,Q0,\<xi>,\<theta>) where:
+----- J0 = {1}
+----- Q0 = P0 = {1,2} 
+----- \<xi> : {1} \<rightarrow> {2}, \<xi>(1) = 2
+----- \<theta> \<subseteq> J0 \<times> Q0 = {1} \<times> {1,2}, \<theta> = {(1,1)} 
+(the binding happens in the first recursve component).   
+*)
+
 
 locale Expression = Nominal +
   fixes Ector :: "('a :: var, 'a, 'e, 'e) G \<Rightarrow> 'e"
@@ -290,8 +116,6 @@ lemma Ector_fresh_inject:
     done
   apply blast
   done
-
-
 
 end
 
