thys/Substitution/Underlying_MN_Monad.thy
@@ -1,0 +1,144 @@
+theory Underlying_MN_Monad
+imports Preliminaries 
+begin
+
+(**************************)
+(* The starting MN-monad / pre-(co)datatype *)
+(* Our G stands for G0 in the 
+triple (I0,P0,G0), where:  
+--- I0 = {1,2} (two variable kinds, represented by the first 
+two Isabelle type-variables 'a1 and 'a2 of ('a1,'a2,'c1,'c2)G);
+--- P0 = {1,2} (two parameter kinds, represented by the first 
+two Isabelle type-variables 'c1 and 'c2 of ('a1,'a2,'c1,'c2)G).
+*)
+
+typedecl Gbd_type
+consts Gbd :: "Gbd_type rel"
+
+setup \<open>Sign.mandatory_path "G"\<close>
+axiomatization where
+  infinite_regular_card_order: "infinite_regular_card_order Gbd"
+setup \<open>Sign.parent_path\<close>
+
+class covar =
+  assumes large: "cardSuc Gbd \<le>o |UNIV::'a set|"
+    and regular: "regularCard |UNIV::'a set|"
+
+class var =
+  assumes large: "|Field Gbd| \<le>o |UNIV::'a set|"
+    and regular: "regularCard |UNIV::'a set|"
+
+instantiation Gbd_type :: var begin
+instance apply standard
+  apply simp
+  by (meson G.infinite_regular_card_order card_of_unique
+      card_order_on_Card_order infinite_regular_card_order_def
+      regularCard_ordIso)
+end
+
+subclass (in covar) var
+  apply standard
+  apply (meson cardSuc_ordLess_ordLeq card_of_Card_order
+      card_of_Field_ordIso G.infinite_regular_card_order
+      infinite_regular_card_order.Card_order local.large
+      ordIso_ordLeq_trans ordLeq_iff_ordLess_or_ordIso)
+  by (rule local.regular)
+
+subclass (in var) infinite
+  apply standard
+  using card_of_ordLeq_finite cinfinite_def
+    G.infinite_regular_card_order
+    infinite_regular_card_order.cinfinite local.large
+  by auto
+
+lemma large': "Gbd \<le>o |UNIV::'a::var set|"
+  using Card_order_iff_ordLeq_card_of var_class.large
+    G.infinite_regular_card_order infinite_regular_card_order.Card_order ordLeq_transitive
+  by blast
+
+lemma (in var) UN_bound: "|A| <o |UNIV::'a set| \<Longrightarrow> (\<And>x. x \<in> A \<Longrightarrow> |f x| <o |UNIV::'a set| )
+  \<Longrightarrow> |\<Union>(f ` A)| <o |UNIV::'a set|"
+  using card_of_Card_order card_of_UNION_ordLess_infinite_Field local.regular regularCard_stable
+  by (metis Field_card_of infinite_UNIV)
+
+lemma IImsupp_bound[simp]:
+  "|SSupp Inj (\<rho> :: 'a::var \<Rightarrow> _)| <o |UNIV :: 'a set| \<Longrightarrow> (\<And>x. |Vr (\<rho> x)| <o |UNIV :: 'a set| ) \<Longrightarrow>
+  |IImsupp' Inj (Vr :: _ \<Rightarrow> 'a set) \<rho>| <o |UNIV :: 'a set|"
+  unfolding IImsupp_def IImsupp'_def
+  by (auto simp: Un_bound UN_bound)
+
+typedecl ('a1, 'a2, 'c1, 'c2) G
+consts Gsub :: "('a1 :: var \<Rightarrow> 'a1) \<Rightarrow> ('a2 :: var \<Rightarrow> 'a2) \<Rightarrow> ('a1, 'a2, 'c1, 'c2) G \<Rightarrow> ('a1, 'a2, 'c1, 'c2) G"
+consts GVrs1 :: "('a1 :: var, 'a2 :: var, 'c1, 'c2) G \<Rightarrow> 'a1 set"
+consts GVrs2 :: "('a1 :: var, 'a2 :: var, 'c1, 'c2) G \<Rightarrow> 'a2 set"
+consts Gmap :: "('c1 \<Rightarrow> 'c1') \<Rightarrow> ('c2 \<Rightarrow> 'c2') \<Rightarrow> ('a1, 'a2, 'c1, 'c2) G \<Rightarrow> ('a1, 'a2, 'c1', 'c2') G"
+consts GSupp1 :: "('a1 :: var, 'a2 :: var, 'c1, 'c2) G \<Rightarrow> 'c1 set"
+consts GSupp2 :: "('a1 :: var, 'a2 :: var, 'c1, 'c2) G \<Rightarrow> 'c2 set"
+
+setup \<open>Sign.mandatory_path "G"\<close>
+
+axiomatization where
+  Sb_Inj: "Gsub id id = id" and
+  Sb_comp: "\<And>g1 g2 f1 f2.
+       |supp (f1 :: 'a1::var \<Rightarrow> 'a1)| <o |UNIV :: 'a1 set| \<Longrightarrow>
+       |supp (f2 :: 'a2::var \<Rightarrow> 'a2)| <o |UNIV :: 'a2 set| \<Longrightarrow>
+       |supp (g1 :: 'a1::var \<Rightarrow> 'a1)| <o |UNIV :: 'a1 set| \<Longrightarrow>
+       |supp (g2 :: 'a2::var \<Rightarrow> 'a2)| <o |UNIV :: 'a2 set| \<Longrightarrow>
+       Gsub g1 g2 \<circ> Gsub f1 f2 = Gsub (g1 \<circ> f1) (g2 \<circ> f2)" and
+  Vrs1_bd: "(\<And>x. |GVrs1 x| <o Gbd)" and
+  Vrs2_bd: "(\<And>x. |GVrs2 x| <o Gbd)" and
+  Vrs1_Sb: "(\<And>f1 f2 x.
+       |supp (f1 :: 'a1::var \<Rightarrow> 'a1)| <o |UNIV :: 'a1 set| \<Longrightarrow>
+       |supp (f2 :: 'a2::var \<Rightarrow> 'a2)| <o |UNIV :: 'a2 set| \<Longrightarrow> GVrs1 (Gsub f1 f2 x) = f1 ` GVrs1 x)" and
+  Vrs2_Sb: "(\<And>f1 f2 x.
+       |supp (f1 :: 'a1::var \<Rightarrow> 'a1)| <o |UNIV :: 'a1 set| \<Longrightarrow>
+       |supp (f2 :: 'a2::var \<Rightarrow> 'a2)| <o |UNIV :: 'a2 set| \<Longrightarrow> GVrs2 (Gsub f1 f2 x) = f2 ` GVrs2 x)" and
+  Sb_cong: "\<And>f1 f2 g1 g2 x.
+       |supp (f1 :: 'a1::var \<Rightarrow> 'a1)| <o |UNIV :: 'a1 set| \<Longrightarrow>
+       |supp (f2 :: 'a2::var \<Rightarrow> 'a2)| <o |UNIV :: 'a2 set| \<Longrightarrow>
+       |supp (g1 :: 'a1::var \<Rightarrow> 'a1)| <o |UNIV :: 'a1 set| \<Longrightarrow>
+       |supp (g2 :: 'a2::var \<Rightarrow> 'a2)| <o |UNIV :: 'a2 set| \<Longrightarrow>
+       (\<And>a1. a1 \<in> GVrs1 x \<Longrightarrow> f1 a1 = g1 a1) \<Longrightarrow>
+       (\<And>a2. a2 \<in> GVrs2 x \<Longrightarrow> f2 a2 = g2 a2) \<Longrightarrow>
+       Gsub f1 f2 x = Gsub g1 g2 x" and
+  Map_id: "Gmap id id = id" and
+  Map_comp: "\<And>f1 f2 g1 g2. Gmap g1 g2 \<circ> Gmap f1 f2 = Gmap (g1 \<circ> f1) (g2 \<circ> f2)" and
+  Supp1_Map: "(\<And>f1 f2 x. GSupp1 (Gmap f1 f2 x) = f1 ` GSupp1 x)" and
+  Supp2_Map: "(\<And>f1 f2 x. GSupp2 (Gmap f1 f2 x) = f2 ` GSupp2 x)" and
+  Supp1_bd: "(\<And>x. |GSupp1 x| <o Gbd)" and
+  Supp2_bd:  "(\<And>x. |GSupp2 x| <o Gbd)" and
+  Map_cong: "\<And>f1 f2 g1 g2 x.
+        (\<And>a. a \<in> GSupp1 x \<Longrightarrow> f1 a = g1 a) \<Longrightarrow>
+        (\<And>a. a \<in> GSupp2 x \<Longrightarrow> f2 a = g2 a) \<Longrightarrow>
+        Gmap f1 f2 x = Gmap g1 g2 x" and
+  Map_Sb: "\<And>f1 f2 g1 g2.
+        |supp (g1 :: 'a1::var \<Rightarrow> 'a1)| <o |UNIV :: 'a1 set| \<Longrightarrow>
+        |supp (g2 :: 'a2::var \<Rightarrow> 'a2)| <o |UNIV :: 'a2 set| \<Longrightarrow>
+        Gmap f1 f2 \<circ> Gsub g1 g2 = Gsub g1 g2 \<circ> Gmap f1 f2" and
+  Supp1_Sb: "(\<And>g1 g2 x.
+        |supp (g1 :: 'a1::var \<Rightarrow> 'a1)| <o |UNIV :: 'a1 set| \<Longrightarrow>
+        |supp (g2 :: 'a2::var \<Rightarrow> 'a2)| <o |UNIV :: 'a2 set| \<Longrightarrow> GSupp1 (Gsub g1 g2 x) = GSupp1 x)" and
+  Supp2_Sb:"(\<And>g1 g2 x.
+        |supp (g1 :: 'a1::var \<Rightarrow> 'a1)| <o |UNIV :: 'a1 set| \<Longrightarrow>
+        |supp (g2 :: 'a2::var \<Rightarrow> 'a2)| <o |UNIV :: 'a2 set| \<Longrightarrow> GSupp2 (Gsub g1 g2 x) = GSupp2 x)" and
+  Vrs_Map1: "(\<And>f1 f2 x. GVrs1 (Gmap f1 f2 x) = GVrs1 x)" and
+  Vrs_Map2: "(\<And>f1 f2 x. GVrs2 (Gmap f1 f2 x) = GVrs2 x)"
+
+lemmas Vrs_Sb = G.Vrs1_Sb G.Vrs2_Sb
+lemmas Vrs_bd = G.Vrs1_bd G.Vrs2_bd
+lemmas Supp_Map = G.Supp1_Map G.Supp2_Map
+lemmas Supp_bd = G.Supp1_bd G.Supp2_bd
+lemmas Supp_Sb = G.Supp1_Sb G.Supp2_Sb
+lemmas Vrs_Map = G.Vrs_Map1 G.Vrs_Map2
+
+setup \<open>Sign.parent_path\<close>
+
+(* In this case the flat version, Gren, happens to be the same as Gsub. *)
+definition Gren :: 
+  "('a1 :: var \<Rightarrow> 'a1) \<Rightarrow> ('a2 :: var \<Rightarrow> 'a2) \<Rightarrow> ('a1, 'a2, 'c1, 'c2) G \<Rightarrow> ('a1, 'a2, 'c1, 'c2) G" where 
+  "Gren \<rho>1 \<rho>2 u = Gsub \<rho>1 \<rho>2 u"
+
+lemma GVrs2_bound[simp]: "|GVrs2 (u::('a :: var, 'a, 'e, 'e) G)| <o |UNIV :: 'a set|"
+  by (rule ordLess_ordLeq_trans[OF G.Vrs_bd(2) large'])
+
+end 
